% !TEX root=main.tex


%% Normalisation %%

\newcommand*{\NPure}
  {\inferrule*[lab=N-Pure]
    { }
    {`v, s \downto `v, s}}

\newcommand*{\NSeqEval}
  {\inferrule*[lab=N-SeqEval,right={$t_1' \neq `v$}]
    {t_1, s \downto t_1', s'}
    {t_1 \Then e, s \downto t_1' \Then e, s'}}

\newcommand*{\NSeq}
  {\inferrule*[lab=N-Seq,right={$t_1' = `v$}]
    {t_1, s \downto t_1', s'   \\
     e\ v \Downarrow t_2       \\
     t_2, s' \downto t_2', s'' }
    {t_1 \Then e, s \downto t_2', s''}}

\newcommand*{\NAndEval}
  {\inferrule*[lab=N-AndEval,right={$t_1' \neq `v_1 \land t_2' \neq `v_2$}]
    {t_1, s  \downto t_1', s'  \\
     t_2, s' \downto t_2', s'' }
    {t_1 \And t_2, s \downto t_1' \And t_2', s}}

\newcommand*{\NAnd}
  {\inferrule*[lab=N-And,right={$t_1' = `v_1 \land t_2' = `v_2$}]
    {t_1, s  \downto t_1', s'  \\
     t_2, s' \downto t_2', s'' }
    {t_1 \And t_2, s \downto \{`v_1, `v_2\}, s}}

\newcommand*{\NOrEval}
  {\inferrule*[lab=N-OrEval]%,right={$t_1' \neq `v_1 \land t_2' \neq `v_2$}]
    {t_1, s  \downto t_1', s'  \\
     t_2, s' \downto t_2', s'' }
    {t_1 \Or t_2, s \downto t_1' \Or t_2', s}}

\newcommand*{\NEdit}
  {\inferrule*[lab=N-Edit]
    { }
    {\Edit v, s \downto \Edit v, s}}

\newcommand*{\NEmpty}
  {\inferrule*[lab=N-Empty]
    { }
    {\Empty, s \downto \Empty, s}}

\newcommand*{\NWatch}
  {\inferrule*[lab=N-Watch]
    { }
    {\Watch l, s \downto \Watch l, s}}

\newcommand*{\NFail}
  {\inferrule*[lab=N-Fail]
    { }
    {\Fail, s \downto \Fail, s}}
